Unfold a bit more to make actions succeed without explode

iodiv/TauIODiv.fst
@@ -68,19 +68,14 @@ effect IODiv (a : Type) (pre : history -> Type0) (post : (hist : history) -> oru
 let act_call (ac : io_sig.act) (x : io_sig.arg ac) : IODIV (io_sig.res x) (iodiv_act ac x) =
   IODIV?.reflect (iodiv_call ac x)
 
-let open_file (s : string) : IODiv file_descr (requires fun hist -> True) (ensures fun hist r -> terminates r /\ ret_trace r == [ EOpenFile s (result r) ])
-// by (compute ())
-// by (norm [delta_only [`%ishift_post ; `%as_iwp ; `%i_bind_post ; `%i_bind_post' ; `%i_pre_le]] ; dump "h") // ishift_post is still present in the goal...
-by (explode ())
-= act_call OpenFile s
+let open_file (s : string) : IODiv file_descr (requires fun hist -> True) (ensures fun hist r -> terminates r /\ ret_trace r == [ EOpenFile s (result r) ]) =
+  act_call OpenFile s
 
-let read (fd : file_descr) : IODiv string (requires fun hist -> is_open fd hist) (ensures fun hist r -> terminates r /\ ret_trace r == [ ERead fd (result r) ])
-by (explode ())
-= act_call Read fd
+let read (fd : file_descr) : IODiv string (requires fun hist -> is_open fd hist) (ensures fun hist r -> terminates r /\ ret_trace r == [ ERead fd (result r) ]) =
+  act_call Read fd
 
-let close (fd : file_descr) : IODiv unit (requires fun hist -> is_open fd hist) (ensures fun hist r -> terminates r /\ ret_trace r == [ EClose fd ])
-by (explode ())
-= act_call Close fd
+let close (fd : file_descr) : IODiv unit (requires fun hist -> is_open fd hist) (ensures fun hist r -> terminates r /\ ret_trace r == [ EClose fd ]) =
+  act_call Close fd
 
 let iter #index #a #w (f : (j : index) -> IODIV (either index a) (w j)) (i : index) : IODIV a (i_iter w i) =
   IODIV?.reflect (dm_iter (fun j -> reify (f j)) i)
