iodiv/DivFreeTauSpec.fst
@@ -634,13 +634,13 @@ let repeat_inv_proof #index (pre : index -> i_pre) (inv : trace -> Type0) (i : i
 (** Unfolding things so that they compute better now that the proofs are done. *)
 
 let pp_unfold l () : Tac unit =
-  norm [delta_only l] ; trefl ()
+  norm [delta_only l ; iota] ; trefl ()
 
 [@@ (postprocess_with (pp_unfold [ `%ile ; `%i_post_le ]))]
 unfold let _ile = ile
 
-[@@ (postprocess_with (pp_unfold [ `%i_ret ]))]
+[@@ (postprocess_with (pp_unfold [ `%i_ret ; `%as_iwp ]))]
 unfold let _i_ret = i_ret
 
-[@@ (postprocess_with (pp_unfold [ `%i_bind ; `%i_bind_post ; `%i_bind_post' ]))]
+[@@ (postprocess_with (pp_unfold [ `%i_bind ; `%i_bind_post ; `%i_bind_post' ; `%as_iwp ]))]
 unfold let _i_bind = i_bind
